Phi_Semantics/PhSem_BC_Storage.thy
@@ -1,10 +1,16 @@
 theory PhSem_BC_Storage
-  imports Phi_System.Resource_Template
+  imports Phi_System.Resource_Template PhSem_MoV
 begin
 
 section \<open>Semantics\<close>
 
+datatype contract = Null | MemBlk nat TY
 
+
+locale BC_storage =
+  partial_map_resource Res \<open>\<lambda>blk. discrete ` Well_Type (typ_of_blk blk)\<close>
+  for Res :: "('blk \<Rightarrow> VAL discrete option) resource_entry"
+  and typ_of_blk :: \<open>'blk \<Rightarrow> TY\<close>
 
 
 end
