Phi_Semantics/PhiSem_Mem_C_Base.thy
@@ -98,209 +98,11 @@ being a tree enabling separation of aggregate structures.
 \<close>
 
 debt_axiomatization Byte_Rep_of_Val :: \<open>VAL \<Rightarrow> 8 word list\<close>
-  where Byte_Rep_of_Val_inj: \<open>Va \<in> Well_Type T \<Longrightarrow> Vb \<in> Well_Type T \<Longrightarrow> Byte_Rep_of_Val Va = Byte_Rep_of_Val Vb \<Longrightarrow> Va = Vb\<close>
+  where Byte_Rep_of_Val_inj': \<open>Va \<in> Well_Type T \<Longrightarrow> Vb \<in> Well_Type T \<Longrightarrow> Byte_Rep_of_Val Va = Byte_Rep_of_Val Vb \<Longrightarrow> Va = Vb\<close>
 
-definition Val_of_Rep_Byte :: \<open>TY \<Rightarrow> 8 word list \<Rightarrow> VAL\<close>
-  where \<open>Val_of_Rep_Byte TY rep = (@v. Byte_Rep_of_Val v = rep \<and> v \<in> Well_Type TY)\<close>
+interpretation Byte: MoV Byte_Rep_of_Val
+  by (standard, rule Byte_Rep_of_Val_inj', assumption, assumption, assumption)
 
-definition map_Rep_Byte :: \<open>TY \<Rightarrow> (VAL \<Rightarrow> VAL) \<Rightarrow> 8 word list \<Rightarrow> 8 word list\<close>
-  where \<open>map_Rep_Byte TY f x = Byte_Rep_of_Val (f (Val_of_Rep_Byte TY x))\<close>
-
-lemma Val_of_Rep_Byte_inj[simp]:
-  \<open> v \<in> Well_Type TY
-\<Longrightarrow> Val_of_Rep_Byte TY (Byte_Rep_of_Val v) = v\<close>
-  unfolding Val_of_Rep_Byte_def
-  using Byte_Rep_of_Val_inj by blast
-
-abbreviation Byte_Rep_of_TY
-  where \<open>Byte_Rep_of_TY TY \<equiv> Byte_Rep_of_Val ` Well_Type TY\<close>
-
-lemma split_Byte_Rep_ExSet:
-  \<open> (\<And>x. P x \<Longrightarrow> x \<in> Byte_Rep_of_TY TY)
-\<Longrightarrow> (A x \<s>\<u>\<b>\<j> x. P x) =
-    (A (Byte_Rep_of_Val v) \<s>\<u>\<b>\<j> v. P (Byte_Rep_of_Val v)) \<close>
-  unfolding BI_eq_iff split_discrete_ex
-  by (auto simp: image_iff Bex_def)
-
-
-definition Byte_Rep_of_Val_ins
-  where \<open>Byte_Rep_of_Val_ins TY = map_option (map_discrete (Val_of_Rep_Byte TY))\<close>
-
-definition Byte_Rep_of_Val_ins_dom
-  where \<open>Byte_Rep_of_Val_ins_dom TY = {x. pred_option (\<lambda>x'. discrete.dest x' \<in> Byte_Rep_of_TY TY) x}\<close>
-
-lemma Byte_Rep_of_Val_ins_eval[simp]:
-  \<open>Byte_Rep_of_Val_ins TY (Some (discrete u)) = (Some (discrete (Val_of_Rep_Byte TY u)))\<close>
-  \<open>Byte_Rep_of_Val_ins TY None = None\<close>
-  unfolding Byte_Rep_of_Val_ins_def by simp+
-
-lemma Byte_Rep_of_Val_ins_dom_eval[simp]:
-  \<open> None \<in> Byte_Rep_of_Val_ins_dom TY \<close>
-  \<open>Some (discrete x) \<in> Byte_Rep_of_Val_ins_dom TY \<longleftrightarrow> x \<in> Byte_Rep_of_TY TY\<close>
-  unfolding Byte_Rep_of_Val_ins_dom_def by simp+
-
-lemma \<F>_functional_condition_Byte_Rep_of_Val_ins_dom:
-  \<open>\<F>_functional_condition (Byte_Rep_of_Val_ins_dom TY)\<close>
-  unfolding \<F>_functional_condition_def Byte_Rep_of_Val_ins_dom_def
-  by(clarsimp; case_tac r; case_tac x; case_tac y; simp)
-
-(*
-interpretation Map_of_Val_ins_UNIV: cancl_sep_orthogonal_monoid \<open>Map_of_Val_ins\<close> UNIV
-  apply (standard; clarsimp simp add: Map_of_Val_ins_def split_discrete_meta_all
-                                      Map_of_Val_ins_dom_def
-                            split: option.split)
-  apply (auto simp add: fun_eq_iff split_option_ex times_fun 
-                                  sep_disj_fun_def split_discrete_meta_all
-                        split: option.split)[1]
-  using Mapof_not_1 apply fastforce *)
-
-
-interpretation Byte_Rep_of_Val_ins: cancl_sep_orthogonal_monoid \<open>Byte_Rep_of_Val_ins TY\<close> \<open>Byte_Rep_of_Val_ins_dom TY\<close>
-  unfolding Byte_Rep_of_Val_ins_def Byte_Rep_of_Val_ins_dom_def
-  by (rule cancl_sep_orthogonal_monoid__map_option_discrete,
-      simp add: inj_on_def split_discrete_all split_option_all, force,
-      simp)
-
-
-
-
-
-context notes mul_carrier_option_def[simp] option.pred_True[simp] begin
-
-lemma fiction_Map_of_Val_perm_partial_refinement_BYTE:
-  \<open> valid_index TY idx
-\<Longrightarrow> v \<in> Well_Type (index_type idx TY)
-\<Longrightarrow> u_idx \<in> Well_Type (index_type idx TY)
-\<Longrightarrow> \<forall>x\<in>Well_Type TY. index_mod_value cidx (\<lambda>_. v) x = index_mod_value idx (\<lambda>_. v) x
-\<Longrightarrow> (\<exists>\<^sup>su. {(Some u, (Some o map_discrete (map_Rep_Byte TY (index_mod_value cidx (\<lambda>_. v)))) u)}
-          \<s>\<u>\<b>\<j>\<s> u \<in> discrete ` Byte_Rep_of_Val ` {a. index_value idx a = u_idx \<and> a \<in> Well_Type TY}
-            \<and> u \<in> discrete ` Byte_Rep_of_Val ` Well_Type TY) * Id_on UNIV
-    \<r>\<e>\<f>\<i>\<n>\<e>\<s> {(to_share o idx \<tribullet>\<^sub>m (map_option discrete \<circ> Map_of_Val u_idx),
-            to_share o idx \<tribullet>\<^sub>m (map_option discrete \<circ> Map_of_Val v))}
-    \<w>.\<r>.\<t> (\<F>_functional (Byte_Rep_of_Val_ins TY) (Byte_Rep_of_Val_ins_dom TY) \<Zcomp>
-          \<F>_functional((\<circ>) to_share \<circ> Map_of_Val_ins) (Map_of_Val_ins_dom TY))
-    \<i>\<n> {to_share o idx \<tribullet>\<^sub>m (map_option discrete \<circ> Map_of_Val u_idx)}\<close>
-  subgoal premises prems proof -
-
-    have simp1: \<open>(\<exists>\<^sup>su. A u \<s>\<u>\<b>\<j>\<s>
-        u \<in> discrete ` Byte_Rep_of_Val ` {a. index_value idx a = u_idx \<and> a \<in> Well_Type TY} \<and> u \<in> discrete ` Byte_Rep_of_TY TY)
-      = (\<exists>\<^sup>sa. A (discrete (Byte_Rep_of_Val a)) \<s>\<u>\<b>\<j>\<s> index_value idx a = u_idx \<and> a \<in> Well_Type TY)\<close>
-      for A
-      unfolding Byte_Rep_of_Val_ins_def
-      by (auto simp: image_iff)
-
-    have simp2: \<open>(\<exists>\<^sup>su. A u \<s>\<u>\<b>\<j>\<s>
-        u \<in> discrete ` {a. index_value idx a = u_idx \<and> a \<in> Well_Type TY} \<and> u \<in> discrete ` Well_Type TY)
-      = (\<exists>\<^sup>sa. A (discrete a) \<s>\<u>\<b>\<j>\<s> index_value idx a = u_idx \<and> a \<in> Well_Type TY)\<close>
-      for A
-      unfolding Byte_Rep_of_Val_ins_def BI_eq_iff
-      by (auto simp: image_iff)
-
-    have t1[simp]:
-      \<open>Domain (\<exists>\<^sup>sa. {(x a, y a)} \<s>\<u>\<b>\<j>\<s> P a) = (\<exists>\<^sup>sa. {(x a)} \<s>\<u>\<b>\<j>\<s> P a)\<close> for x y P
-      unfolding set_eq_iff
-      by auto
-
-    have simp3[simp]:
-         \<open>a \<in> Well_Type TY
-       \<Longrightarrow> Val_of_Rep_Byte TY (map_Rep_Byte TY (index_mod_value cidx (\<lambda>_. v)) (Byte_Rep_of_Val a))
-         = index_mod_value idx (\<lambda>_. v) a \<close> for a
-      by (simp add: index_mod_value_welltyp map_Rep_Byte_def prems(1) prems(2) prems(4))
-      
-
-    note [cong] = SubjectionSet_cong
-
-    note [simp] = ExSet_image SubjectionSet_image
-
-    note t11 = refinement_frame[where R = UNIV, OF Byte_Rep_of_Val_ins.\<F>_functional_refinement_complex,
-        where R4=\<open>\<exists>\<^sup>sa. {(Some (discrete (Byte_Rep_of_Val a)), Some (discrete (map_Rep_Byte TY (index_mod_value cidx (\<lambda>_. v)) (Byte_Rep_of_Val a))))}
-                  \<s>\<u>\<b>\<j>\<s> index_value idx a = u_idx \<and> a \<in> Well_Type TY\<close>
-          and TY4 = TY,
-       simplified]
-
-    show ?thesis
-    apply (insert prems,
-          rule sep_refinement_stepwise)
-    prefer 2
-    apply (rule fiction_Map_of_Val_perm_partial_refinement)
-    apply (assumption)
-    apply (assumption)
-    apply (assumption)
-    apply (assumption)
-    apply (simp add: simp1 simp2)
-    apply (rule t11)
-    apply (clarsimp simp: )
-          using index_mod_value_welltyp map_Rep_Byte_def apply force
-    apply (clarsimp simp: frame_preserving_relation_def)
-    apply (simp add: Sep_Closed_def \<F>_functional_comp)
-    apply (rule subset_trans[OF fiction_Map_of_Val_ins_perm_projection])
-    apply blast
-    apply blast
-    by (clarsimp simp: set_mult_expn)
-qed .
-
-lemma fiction_Map_of_Val_ins_perm_projection_BYTE:
-  \<open> valid_index TY idx
-\<Longrightarrow> u_idx \<in> Well_Type (index_type idx TY)
-\<Longrightarrow> refinement_projection
-      (\<F>_functional (Byte_Rep_of_Val_ins TY) (Byte_Rep_of_Val_ins_dom TY) \<Zcomp>
-       \<F>_functional ((\<circ>) to_share o Map_of_Val_ins) (Map_of_Val_ins_dom TY))
-      { to_share o idx \<tribullet>\<^sub>m (map_option discrete \<circ> Map_of_Val u_idx) }
-    \<subseteq> Some ` discrete ` Byte_Rep_of_Val ` {a. index_value idx a = u_idx \<and> a \<in> Well_Type TY } * UNIV \<close>
-subgoal premises prems proof -
-  have t1:
-       \<open>Byte_Rep_of_Val_ins TY ` Some ` discrete ` Byte_Rep_of_Val ` {a. index_value idx a = u_idx \<and> a \<in> Well_Type TY}
-      = Some ` discrete ` {a. index_value idx a = u_idx \<and> a \<in> Well_Type TY}\<close>
-    for TY
-    by (auto simp add: image_iff)
-  show ?thesis
-  apply (rule refinement_projections_stepwise_UNIV_paired)
-  prefer 2
-  apply (rule fiction_Map_of_Val_ins_perm_projection, insert prems)
-  apply (assumption)
-  apply (assumption)
-  apply (rule Byte_Rep_of_Val_ins.\<F>_functional_projection[
-          where S=\<open>Some ` discrete ` Byte_Rep_of_Val ` {a. index_value idx a = u_idx \<and> a \<in> Well_Type TY}\<close>
-            and TY=TY,
-          simplified t1])
-  apply (clarsimp) .
-qed .
-
-lemma fiction_Map_of_Val_ins_perm_projection_half_BYTE:
-  \<open> valid_index TY idx
-\<Longrightarrow> u_idx \<in> Well_Type (index_type idx TY)
-\<Longrightarrow> 0 < n
-\<Longrightarrow> refinement_projection
-     (\<F>_functional (Byte_Rep_of_Val_ins TY) (Byte_Rep_of_Val_ins_dom TY) \<Zcomp>
-      \<F>_functional ((\<circ>) to_share \<circ> Map_of_Val_ins) (Map_of_Val_ins_dom TY))
-      { n \<odivr> (to_share o idx \<tribullet>\<^sub>m (map_option discrete \<circ> Map_of_Val u_idx)) }
-   \<subseteq> Some ` discrete ` Byte_Rep_of_Val ` {a. index_value idx a = u_idx \<and> a \<in> Well_Type TY} * UNIV\<close>
-  subgoal premises prems proof -
-  
-  have t1:
-      \<open>(Byte_Rep_of_Val_ins TY ` Some ` discrete ` Byte_Rep_of_Val ` {a. index_value idx a = u_idx \<and> a \<in> Well_Type TY})
-     = (Some ` discrete ` {a. index_value idx a = u_idx \<and> a \<in> Well_Type TY})\<close>
-      unfolding Byte_Rep_of_Val_ins_def set_eq_iff
-      by (auto simp: image_iff)
-
- show ?thesis
-  by (insert prems,
-      rule refinement_projections_stepwise_UNIV_paired,
-      rule Byte_Rep_of_Val_ins.\<F>_functional_projection
-        [where S=\<open>Some ` discrete ` Byte_Rep_of_Val ` {a. index_value idx a = u_idx \<and> a \<in> Well_Type TY}\<close>,
-          where TY=TY,
-          simplified t1],
-      ((auto simp: Byte_Rep_of_Val_ins_dom_def)[1]),
-      rule fiction_Map_of_Val_ins_perm_projection_half,
-      assumption,
-      assumption,
-      assumption)
-qed .
-
-end
-
-lemma split_discrete_ExBI: \<open>(\<exists>*x. P x) = (\<exists>*x. P (discrete x))\<close>
-  unfolding BI_eq_iff by (simp add: split_discrete_ex)
 
 locale aggregate_mem_resource =
   partial_map_resource Res \<open>\<lambda>blk. discrete ` Byte_Rep_of_Val ` Well_Type (typ_of_blk blk)\<close>
@@ -309,7 +111,7 @@ locale aggregate_mem_resource =
 
 locale perm_aggregate_mem_fiction =
   pointwise_base_fiction_for_partial_mapping_resource
-      Res \<open>\<lambda>blk. \<F>_functional (Byte_Rep_of_Val_ins (typ_of_blk blk)) (Byte_Rep_of_Val_ins_dom (typ_of_blk blk)) \<Zcomp>
+      Res \<open>\<lambda>blk. \<F>_functional (Byte.Rep_of_Val_ins (typ_of_blk blk)) (Byte.Rep_of_Val_ins_dom (typ_of_blk blk)) \<Zcomp>
                  \<F>_functional ((\<circ>) to_share \<circ> Map_of_Val_ins) (Map_of_Val_ins_dom (typ_of_blk blk))\<close>
       Fic \<open>\<lambda>blk. discrete ` Byte_Rep_of_Val ` Well_Type (typ_of_blk blk)\<close>
   for Res :: "('blk \<Rightarrow> 8 word list discrete option) resource_entry"
@@ -334,23 +136,19 @@ lemma getter_rule:
     by (simp add: prems(2))
 
   have simp1: \<open>
-      (A x \<s>\<u>\<b>\<j> x. B x \<and> x \<in> Byte_Rep_of_TY (typ_of_blk blk) \<and> x \<in> Byte_Rep_of_Val ` {a. index_value idx a = u_idx \<and> a \<in> Well_Type (typ_of_blk cblk)})
+      (A x \<s>\<u>\<b>\<j> x. B x \<and> x \<in> Byte.Rep_of_TY (typ_of_blk blk) \<and> x \<in> Byte_Rep_of_Val ` {a. index_value idx a = u_idx \<and> a \<in> Well_Type (typ_of_blk cblk)})
     = (A (Byte_Rep_of_Val v) \<s>\<u>\<b>\<j> v. B (Byte_Rep_of_Val v) \<and> v \<in> Well_Type (typ_of_blk blk) \<and> index_value idx v = u_idx) \<close>
   for A B C ret TY S
   unfolding BI_eq_iff split_discrete_ex
   by (auto simp: image_iff Bex_def)
 
   show ?thesis
-    by (rule "_getter_rule_2_"[OF _ fiction_Map_of_Val_ins_perm_projection_half_BYTE,
+    by (rule "_getter_rule_2_"[OF _ Byte.fiction_Map_of_Val_ins_perm_projection_half_BYTE,
               where k=cblk and k'=blk and idx1=idx and u_idx1=u_idx,
               simplified split_discrete_ExBI inj_image_mem_iff inj_discrete simp1],
         insert prems, simp+)
 qed .
 
-lemma defined_set_in_image[simp]:
-  \<open> { f u' |u'. u' \<in> h ` S} = { f (h u) |u. u \<in> S } \<close>
-  unfolding set_eq_iff
-  by auto
 
 context notes mul_carrier_option_def[simp] option.pred_True[simp] begin
 
@@ -365,20 +163,20 @@ lemma allocate_rule:
 
   note pointwise_set_UNIV[simp] \<F>_functional_condition_Map_of_Val_ins_dom[simp]
 
-  have t1[simp]: \<open>v \<in> U \<Longrightarrow> Val_of_Rep_Byte TY (Byte_Rep_of_Val v) = v\<close> for v
+  have t1[simp]: \<open>v \<in> U \<Longrightarrow> Byte.Val_of_Rep TY (Byte_Rep_of_Val v) = v\<close> for v
     using prems(2) by auto
   have [simp]:
-       \<open>{(1, to_share \<circ> (map_option discrete \<circ> Map_of_Val (Val_of_Rep_Byte TY (Byte_Rep_of_Val v)))) |v. v \<in> U}
+       \<open>{(1, to_share \<circ> (map_option discrete \<circ> Map_of_Val (Byte.Val_of_Rep TY (Byte_Rep_of_Val v)))) |v. v \<in> U}
       = {(1, to_share \<circ> (map_option discrete \<circ> Map_of_Val v)) |v. v \<in> U}\<close>
     by force
 
   note rule = sep_refinement_stepwise[
-        OF refinement_frame[OF Byte_Rep_of_Val_ins.\<F>_functional_refinement'[simplified]]
+        OF refinement_frame[OF Byte.Rep_of_Val_ins.\<F>_functional_refinement'[simplified]]
            sep_refinement_stepwise[
                     OF refinement_frame[OF Map_of_Val_ins.\<F>_functional_refinement'[simplified]]
                        pointwise_to_share.\<F>_functional_refinement'[where B=\<open>Map_of_Val_ins ` B\<close> for B, unfolded defined_set_in_image]
                        pointwise_to_share.\<F>_functional_projection,
-                    where B6=\<open>Byte_Rep_of_Val_ins TY ` B\<close> for B, unfolded defined_set_in_image],
+                    where B6=\<open>Byte.Rep_of_Val_ins TY ` B\<close> for B, unfolded defined_set_in_image],
         where a35=\<open>None\<close> and B22=\<open>{Some (discrete (Byte_Rep_of_Val v)) |v. v \<in> U}\<close>,
         simplified,
         OF _ _ _ refinement_projections_stepwise_UNIV_paired[
@@ -394,8 +192,8 @@ lemma allocate_rule:
         unfold \<F>_functional_comp[where f=\<open>(\<circ>) to_share\<close> and Df=\<open>UNIV\<close>, simplified, simp]
                one_option_def,
         simp, rule rule,
-        simp add: subset_iff, insert Byte_Rep_of_Val_ins_dom_eval(2) prems(2), blast,
-        simp add: \<F>_functional_condition_Byte_Rep_of_Val_ins_dom,
+        simp add: subset_iff, insert Byte.Rep_of_Val_ins_dom_eval(2) prems(2), blast,
+        simp add: Byte.\<F>_functional_condition_Rep_of_Val_ins_dom,
         simp add: subset_iff, force,
         simp add: R.in_invariant inj_image_mem_iff, force,
         clarsimp simp add: R.in_invariant Ball_def dom1_dom, metis dom_map_option_comp prems(1))
@@ -407,18 +205,18 @@ lemma setter_rule:
       \<Longrightarrow> \<p>\<r>\<e>\<m>\<i>\<s>\<e> v \<in> Well_Type (index_type idx (typ_of_blk blk))
       \<Longrightarrow> \<p>\<r>\<e>\<m>\<i>\<s>\<e> u_idx \<in> Well_Type (index_type idx (typ_of_blk blk))
       \<Longrightarrow> \<p>\<r>\<e>\<m>\<i>\<s>\<e> (\<forall>x\<in>Well_Type (typ_of_blk blk). index_mod_value cidx (\<lambda>_. v) x = index_mod_value idx (\<lambda>_. v) x)
-      \<Longrightarrow> \<p>\<r>\<o>\<c> R.\<phi>R_set_res (map_fun_atS cblk (\<lambda>h. {Some (map_discrete (map_Rep_Byte (typ_of_blk cblk) (index_mod_value cidx (\<lambda>_. v))) (the h))}))
+      \<Longrightarrow> \<p>\<r>\<o>\<c> R.\<phi>R_set_res (map_fun_atS cblk (\<lambda>h. {Some (map_discrete (Byte.map_Rep (typ_of_blk cblk) (index_mod_value cidx (\<lambda>_. v))) (the h))}))
             \<lbrace> 1(blk := to_share \<circ> idx \<tribullet>\<^sub>m (map_option discrete \<circ> Map_of_Val u_idx)) \<Ztypecolon> \<phi> Itself \<longmapsto>
               \<lambda>\<r>\<e>\<t>. 1(blk := to_share \<circ> idx \<tribullet>\<^sub>m (map_option discrete \<circ> Map_of_Val v)) \<Ztypecolon> \<phi> Itself \<rbrace> \<close>
   unfolding Premise_def
   by (simp add: EQ[unfolded Premise_def],
-      rule "_setter_rule_2_"[where f=\<open>\<lambda>h. {Some (map_discrete (map_Rep_Byte (typ_of_blk blk) (index_mod_value cidx (\<lambda>_. v))) h)}\<close>
+      rule "_setter_rule_2_"[where f=\<open>\<lambda>h. {Some (map_discrete (Byte.map_Rep (typ_of_blk blk) (index_mod_value cidx (\<lambda>_. v))) h)}\<close>
                         and V=\<open>discrete ` Byte_Rep_of_Val ` {a. index_value idx a = u_idx \<and> a \<in> Well_Type (typ_of_blk blk)}\<close>
                         and F=\<open>\<lambda>_. {to_share o idx \<tribullet>\<^sub>m (map_option discrete \<circ> Map_of_Val v)}\<close>
                         for idx cidx v u_idx,
                       simplified,
-                      OF _ fiction_Map_of_Val_perm_partial_refinement_BYTE[simplified]
-                           fiction_Map_of_Val_ins_perm_projection_BYTE[simplified]],
+                      OF _ Byte.fiction_Map_of_Val_perm_partial_refinement_BYTE[simplified]
+                           Byte.fiction_Map_of_Val_ins_perm_projection_BYTE[simplified]],
       simp,
       assumption,
       assumption,
@@ -427,7 +225,7 @@ lemma setter_rule:
       assumption,
       assumption,
       clarsimp simp add: split_discrete_meta_all inj_image_mem_iff index_mod_value_welltyp image_iff Bex_def,
-      metis Val_of_Rep_Byte_inj index_mod_value_welltyp map_Rep_Byte_def)
+      metis Byte.Val_of_Rep_inj index_mod_value_welltyp Byte.map_Rep_def)
 
 lemma deallocate_rule:
   \<open> \<p>\<r>\<e>\<m>\<i>\<s>\<e> v \<in> Well_Type (typ_of_blk blk)
@@ -444,7 +242,7 @@ proof -
   note inj_image_mem_iff[simp] pointwise_set_UNIV[simp] \<F>_functional_condition_Map_of_Val_ins_dom[simp]
        \<F>_functional_comp[where f=\<open>(\<circ>) to_share\<close> and Df=\<open>UNIV\<close>, simplified, symmetric, simp]
 
-  have [simp]: \<open>Val_of_Rep_Byte (typ_of_blk blk) (Byte_Rep_of_Val v) = v\<close>
+  have [simp]: \<open>Byte.Val_of_Rep (typ_of_blk blk) (Byte_Rep_of_Val v) = v\<close>
     by (simp add: prems)
 
   note rule1 = refinement_projections_stepwise_UNIV_paired[
@@ -459,7 +257,7 @@ apply (rule "_setter_rule_2_"[where f=\<open>\<lambda>_. {None}\<close> and V=\<
 apply (simp,
         unfold refinement_source_subjection, rule impI,
         rule sep_refinement_stepwise [
-            OF refinement_frame[OF Byte_Rep_of_Val_ins.\<F>_functional_refinement[simplified]]
+            OF refinement_frame[OF Byte.Rep_of_Val_ins.\<F>_functional_refinement[simplified]]
                sep_refinement_stepwise[
                         OF refinement_frame[OF Map_of_Val_ins.\<F>_functional_refinement[simplified]]
                            pointwise_to_share.\<F>_functional_refinement
@@ -467,7 +265,7 @@ apply (simp,
             where a16=\<open>Some (discrete (Byte_Rep_of_Val v))\<close> and b16=None and TY16=\<open>typ_of_blk blk\<close>,
             simplified])
     apply blast
-    using \<F>_functional_condition_Byte_Rep_of_Val_ins_dom apply presburger
+    using Byte.\<F>_functional_condition_Rep_of_Val_ins_dom apply presburger
     using prems apply blast
     apply (rule rule1)
     using prems apply blast
@@ -475,7 +273,7 @@ apply (simp,
     prefer 2
     apply (rule rule1)
     apply (simp add: prems)
-    apply (rule Byte_Rep_of_Val_ins.\<F>_functional_projection
+    apply (rule Byte.Rep_of_Val_ins.\<F>_functional_projection
       [where S=\<open>{Some (discrete (Byte_Rep_of_Val v))}\<close> and TY=\<open>typ_of_blk blk\<close>, simplified])
     using prems by blast
 qed .
